utilsTheory.sml
@@ -12,12 +12,10 @@ struct
   local open listTheory
   in end;
   val _ = Theory.link_parents
-          ("utils",
-          Arbnum.fromString "1388583099",
-          Arbnum.fromString "878680")
+          ("utils",Arbnum.fromString "1388649610",Arbnum.fromString "5187")
           [("list",
-           Arbnum.fromString "1380541561",
-           Arbnum.fromString "111594")];
+           Arbnum.fromString "1378778539",
+           Arbnum.fromString "899441")];
   val _ = Theory.incorporate_types "utils" [];
 
   val idvector = 
